Finish up all other async ops

Wavelet/Compile/AffineChan.lean
@@ -7,22 +7,10 @@ open Semantics
 def AtomicProc.inputs [Arity Op] : AtomicProc Op χ V → List χ
   | .op _ inputs _ => inputs.toList
   | .async _ inputs _ => inputs.toList
-  | .merge _ inputs₁ inputs₂ _ => (inputs₁ ++ inputs₂).toList
-  | .forward inputs _ => inputs.toList
-  | .fork input _ => [input]
-  | .const _ act _ => [act]
-  | .forwardc inputs _ _ => inputs.toList
-  | .sink inputs => inputs.toList
 
 def AtomicProc.outputs [Arity Op] : AtomicProc Op χ V → List χ
   | .op _ _ outputs => outputs.toList
   | .async _ _ outputs => outputs.toList
-  | .merge _ _ _ outputs => outputs.toList
-  | .forward _ outputs => outputs.toList
-  | .fork _ outputs => outputs.toList
-  | .const _ _ outputs => outputs.toList
-  | .forwardc _ _ outputs => outputs.toList
-  | .sink _ => []
 
 /-- Each channel name is used at most once. -/
 def AtomicProcs.AffineChan [Arity Op] (aps : AtomicProcs Op χ V) : Prop
