Wavelet/Compile/MapChans.lean
@@ -9,13 +9,6 @@ open Semantics
 def AtomicProc.mapChans [Arity Op] (f : χ → χ') : AtomicProc Op χ V → AtomicProc Op χ' V
   | .op o inputs outputs => .op o (inputs.map f) (outputs.map f)
   | .async aop inputs outputs => .async aop (inputs.map f) (outputs.map f)
-  | .merge decider inputs₁ inputs₂ outputs =>
-    .merge (f decider) (inputs₁.map f) (inputs₂.map f) (outputs.map f)
-  | .forward inputs outputs => .forward (inputs.map f) (outputs.map f)
-  | .fork input outputs => .fork (f input) (outputs.map f)
-  | .const c act outputs => .const c (f act) (outputs.map f)
-  | .forwardc inputs consts outputs => .forwardc (inputs.map f) consts (outputs.map f)
-  | .sink inputs => .sink (inputs.map f)
 
 def AtomicProcs.mapChans [Arity Op] (f : χ → χ')
   : AtomicProcs Op χ V → AtomicProcs Op χ' V
